## The PWKSO ontology for representing possible worlds and Kripke structures

@base <http://ns.inria.fr/pwkso/> .
@prefix : <> .
@prefix owl: <http://www.w3.org/2002/07/owl#> .
@prefix rdf: <http://www.w3.org/1999/02/22-rdf-syntax-ns#> .
@prefix xml: <http://www.w3.org/XML/1998/namespace> .
@prefix xsd: <http://www.w3.org/2001/XMLSchema#> .
@prefix rdfs: <http://www.w3.org/2000/01/rdf-schema#> .
@prefix cc: <http://creativecommons.org/ns#> .
@prefix vann: <http://purl.org/vocab/vann/> .
@prefix dct: <http://purl.org/dc/terms/> .

: a owl:Ontology ;
    dct:title "Possible Worlds and Kripke Structures Ontology"@en ;
    dct:description  "an ontology for representing possible worlds and Kripke structures."@en ;
    cc:license <https://creativecommons.org/licenses/by/4.0/> ;
    vann:preferredNamespacePrefix "pwkso" ;
    vann:preferredNamespaceUri : .
    
:PossibleWorld a owl:Class ;
    rdfs:label "possible world"@en;
    rdfs:comment "a consistent representation of how the world is, could have been or would be"@en .

:verifiedIn a owl:ObjectProperty ;
    rdfs:label "verified in"@en;
    rdfs:comment "links triples to a possible world in which their associated formula is verified"@en;
    rdfs:range :PossibleWorld ;
    owl:propertyDisjointWith :notVerifiedIn .

:notVerifiedIn a owl:ObjectProperty ;
    rdfs:label "not verified in"@en;
    rdfs:comment "links triples to a possible world in which associated formula is not verified"@en;
    rdfs:range :PossibleWorld ;
    owl:propertyDisjointWith :verifiedIn .

## Closed vs open possible worlds

:ClosedPossibleWorld a owl:Class ;
    rdfs:subClassOf :PossibleWorld ;
    rdfs:label "closed possible world"@en;
    rdfs:comment "represents a possible world with the Closed-World Assumption"@en .

:OpenPossibleWorld a owl:Class ;
    rdfs:subClassOf :PossibleWorld ;
    rdfs:label "open possible world"@en;
    rdfs:comment "represents a possible world with the Open-World Assumption"@en .


## Representation using the (N+1)-ary pattern: Introducing a new class for a relation with a distinguished participant

:KripkeRelation a owl:Class ;
    rdfs:label "Kripke relation"@en;
    rdfs:comment "represents the Kripke relations between possible worlds. Instances of :KripkeRelation are recommended to be represented as blank nodes"@en .

:param a owl:ObjectProperty ;
    rdfs:label "parameter"@en;
    rdfs:comment "parameter of a Kripke relation"@en;
    rdfs:domain :KripkeRelation ;
    rdfs:range :PossibleWorld .

:index a owl:ObjectProperty ;
    rdfs:label "index"@en;
    rdfs:comment "index of a Kripke relation"@en;
    rdfs:domain :KripkeRelation .

:hasRelation a owl:ObjectProperty ;
    rdfs:label "has relation"@en;
    rdfs:comment "links a possible world to one of its N-ary relations"@en;
    rdfs:domain :PossibleWorld ;
    rdfs:range :KripkeRelation .
       
:BinaryKripkeRelation 
    rdfs:label "binary Kripke relation"@en;
    rdfs:comment "relation that links a possible world with another to represent a unary modal operator"@en;
    rdfs:subClassOf :KripkeRelation,
     [ a owl:Restriction ;
       owl:cardinality 1 ;
       owl:onProperty :param ] .
       
:UnaryKripkeRelation
    rdfs:label "unary Kripke relation"@en;
    rdfs:comment "relation that links a possible world with another to represent a nullary modal operator"@en;
    rdfs:subClassOf :KripkeRelation,
     [ a owl:Restriction ;
       owl:cardinality 0 ;
       owl:onProperty :param ] .